\begin{figure}
\begin{grammar}
<contr> ::= <contr-stmt> <contr> | <contr-stmt>

<contr-stmt> ::= `guarantee' <STR> `:' <expr> `;'
\alt `assume' <STR> `:' <expr> `;'
\alt `initially' `:' <expr> `;'
\alt <eq-stmt>
\alt <node-stmt>

<impl> ::= <impl-stmt> <impl> | <impl-stmt>

<impl-stmt> ::= `assert' <expr> `;'
\alt `synchrony' `:' <INT-LIT> (`no_simult')? `;'
\alt `lemma' <STR> `:' <expr> `;'
\alt <eq-stmt>
\alt <node-stmt>

<eq-stmt> ::= `eq' <arg-lst> `=' <expr> `;'
\alt `eq' <arg-lst> `;'

<node-stmnt> ::= `node' <ID> `(' <arg-lst> `)' \\
`returns' `(' <arg-lst> `)' `;' \\
(`var' <arg-lst>)? \\
`let' <eq-lst> `tel' `;'

<expr> ::= <BOOL-LIT>
\alt <INT-LIT>
\alt <REAL-LIT>
\alt <ID>
\alt <ID> `(' <expr-lst> `)'
\alt `pre' `(' <expr> `)'
\alt `event' `(' <ID> `)'
\alt `floor' `(' <expr> `)'
\alt `real' `(' <expr> `)'
\alt `Get_Property' `(' <expr> `,' <aadl-property> `)'
\alt `-' <expr>
\alt `not' <expr>
\alt <expr> `{' <ID> `:=' <expr> `}'
\alt <expr> (`*'|`/'|`mod'|`+'|`-') <expr>
\alt <expr> (`<'|`<='|`>'|`>='|`='|`!=') <expr>
\alt <expr> (`and'|`or') <expr>
\alt <expr> `=>' <expr>
\alt <expr> `->' <expr>

<type> ::= `int' | `real' | `bool' | <aadl-type>

<arg-lst> ::= <ID> `:' <type> `,' <arg-lst> | <ID> `:' <type>

<eq-lst> ::= <eq-stmt> <eq-lst> | <eq-stmt>

<expr-lst> ::= <expr> `,' <expr-lst> | <expr>

\end{grammar}
\caption{A simplified description of the grammar for AGREE}
\label{fig:grammar}
\end{figure}